To find the derivative of the function \( f(x) = \sqrt{x}(x^{-1/2} - x^{-3/2})e^{3x} \), we'll use the product rule, the chain rule, and the power rule.

### Simplifying the Function

First, let's simplify the function:

\[ f(x) = \sqrt{x}(x^{-1/2} - x^{-3/2})e^{3x} \]

Recall that \( \sqrt{x} = x^{1/2} \). We can rewrite the function as:

\[ f(x) = x^{1/2} (x^{-1/2} - x^{-3/2}) e^{3x} \]

Let's distribute \( x^{1/2} \) inside the parentheses:

\[ f(x) = x^{1/2} \cdot x^{-1/2} - x^{1/2} \cdot x^{-3/2} \]
\[ f(x) = x^{(1/2 - 1/2)} - x^{(1/2 - 3/2)} \]
\[ f(x) = x^0 - x^{-1} \]
\[ f(x) = 1 - x^{-1} \]

So the function simplifies to:

\[ f(x) = (1 - x^{-1})e^{3x} \]

### Applying the Product Rule

The function is now a product of two functions: \( u(x) = 1 - x^{-1} \) and \( v(x) = e^{3x} \). To find the derivative \( f'(x) \), we will use the product rule:

\[ (uv)' = u'v + uv' \]

#### Step 1: Find \( u'(x) \)

\[ u(x) = 1 - x^{-1} \]
\[ u'(x) = 0 - (-1)x^{-2} \]
\[ u'(x) = x^{-2} \]

#### Step 2: Find \( v'(x) \)

\[ v(x) = e^{3x} \]
Using the chain rule:
\[ v'(x) = e^{3x} \cdot \frac{d}{dx}(3x) \]
\[ v'(x) = 3e^{3x} \]

#### Step 3: Combine using the Product Rule

Now, using the product rule:

\[ f'(x) = u'v + uv' \]
\[ f'(x) = x^{-2} \cdot e^{3x} + (1 - x^{-1}) \cdot 3e^{3x} \]

#### Step 4: Simplify

\[ f'(x) = x^{-2}e^{3x} + 3(1 - x^{-1})e^{3x} \]
\[ f'(x) = x^{-2}e^{3x} + 3e^{3x} - 3x^{-1}e^{3x} \]
\[ f'(x) = e^{3x} \left( x^{-2} + 3 - 3x^{-1} \right) \]

### Final Answer

\[ f'(x) = e^{3x} \left( x^{-2} + 3 - 3x^{-1} \right) \]

So, the derivative of \( f(x) = \sqrt{x}(x^{-1/2} - x^{-3/2})e^{3x} \) is:

\[ f'(x) = e^{3x} \left( x^{-2} + 3 - 3x^{-1} \right) \]

$END$
